src/Examples/MailServer/MailAPI.v
@@ -164,10 +164,12 @@ Module Mail.
     end.
 
   Definition crash_step : relation State State unit :=
-    puts (set open (λ _, false)).
+    _ <- puts (set open (λ _, false));
+    puts (set heap (λ _, ∅)).
 
   Definition finish_step : relation State State unit :=
-    puts (set open (λ _, false)).
+    _ <- puts (set open (λ _, false));
+    puts (set heap (λ _, ∅)).
 
   Definition sem : Dynamics Op State :=
     {| Proc.step := step;
@@ -189,7 +191,9 @@ Module Mail.
     - do 3 eexists; split; econstructor.
     - do 3 eexists; split; econstructor.
     - destruct ret; inversion H; eauto.
+      repeat deex. inversion H1.
     - destruct ret; inversion H; eauto.
+      repeat deex. inversion H1.
   Defined.
 
   End GoModel.
