src/Examples/MailServer/MailRefinement.v
@@ -175,7 +175,7 @@ Proof.
     iLöb as "IH" forall (i Hlen).
     wp_loop.
     destruct equal as [Heqlen|Hneq].
-    - subst.
+    - iClear "IH". subst.
       rewrite firstn_all.
       (* in a sense we do not even need to argue that the spool dir is actually empty at
          this point, it is totally irrelevant *)
@@ -201,6 +201,8 @@ Proof.
       { eauto. }
       iSplitL "Hmsgs".
       { by iApply MsgsInv_crash_set_false. }
+      iSplitL "".
+      { iModIntro. by iApply big_sepDM_empty. }
       iExists _. by iFrame.
     - wp_bind.
       destruct (nth_error ltmps i) as [curr_name|] eqn:Heq_curr_name; last first.
@@ -335,30 +337,76 @@ Proof.
   }
   {
     iIntros (??) "H".
-    iDestruct "H" as (hGtmp) "Hrest".
-    iDestruct "Hrest" as (Γ γ) "(#Hsource&#Hinv)".
+    iDestruct "H" as (hGtmp_old) "Hrest".
+    iDestruct "Hrest" as (Γold γold) "(#Hsource&#Hinv)".
+
     iInv "Hinv" as "H" "_".
     iDestruct "H" as (σ) "(>Hstate&Hmsgs&>Hheap&>Htmp)".
     iApply (fupd_mask_weaken _ _).
     { solve_ndisj. }
     iDestruct "Hmsgs" as (?) "(_&>Hroot&Hinit&Hmsgs)".
+    iDestruct (big_sepM_mono with "Hmsgs") as "Hmsgs".
+    { iIntros (???). iApply MsgInv_weaken. }
+    iDestruct "Hmsgs" as ">Hmsgs".
     iIntros (?????) "(Hroot'&Hglobal)".
     iDestruct "Hroot'" as (S) "(Hroot'&Hdirlocks)".
     iDestruct "Hroot" as "(Hroot&%)".
     iDestruct (ghost_var_agree2 (A := discreteC (gset string))_ with "Hroot Hroot'") as %Heq_dom.
+
+
+    iDestruct "Htmp" as (tmp_map) "(Hdir&_&_&Hpaths)".
+    iMod (gen_heap_init (tmp_map: gmap string Inode)) as (hGTmp) "Htmp".
+    iMod (ghost_var_alloc (A := @ghost_init_statusC gm Hgmwf) Uninit) as "H".
+    iDestruct "H" as (γ) "(Hauth&Hfrag)".
+    iMod (ghost_var_bulk_alloc (A := contentsC) (σ.(messages)) (λ _ _, ∅)) as "H".
+    iDestruct "H" as (Γ HΓdom) "HΓ".
+    iAssert ([∗ map] k↦_ ∈ σ.(messages), ∃ γ0 : gname, ⌜Γ !! k = Some γ0⌝)%I
+            with "[HΓ]" as "#HΓ'".
+    { iApply big_sepM_mono; last eauto. iIntros (???) "H". iDestruct "H" as (?) "(?&?)"; eauto. }
+
     iModIntro.
-    iExists _, _, _. iFrame.
-    iDestruct "Htmp" as (tmps_map) "(Hspool&_&Htmps&Hpaths)".
+    iExists Γ, γ, _. iFrame.
     replace 0%Z with (O : Z) by auto.
-    iDestruct (read_split_join with "Hspool") as "(Hspool1&Hspool2)".
+    iDestruct (read_split_join with "Hdir") as "(Hspool1&Hspool2)".
     rewrite <-Heq_dom.
-    (*
+    iDestruct (big_sepS_delete with "Hdirlocks") as "(Hspoollock&Hdirlocks)".
+    { by apply elem_of_union_r, elem_of_singleton. }
     iSplitR "Hspool2 Hspoollock"; last first.
-    { iExists _. iFrame.
-      replace 0%Z with (O : Z) by auto.
-      iFrame.
-     *)
-    admit.
+    { iExists _. iFrame. }
+    iExists [].
+    rewrite /HeapInv.
+    iSplitR "Htmp Hspool1 Hpaths"; last first.
+    { iSplitL ""; auto.
+      iExists _. iFrame. }
+    iSplitL ""; auto.
+    iSplitL "HΓ".
+    {  iApply big_sepM_mono; last (iApply "HΓ").
+       iIntros (???) "H".
+       iDestruct "H" as (γuid ?) "(?&?)".
+       iExists _. iSplitL ""; auto.
+       iExists _, _. iFrame.
+    }
+    iClear "Hheap".
+    assert (((set_map UserDir (dom (gset uint64) σ.(messages)) ∪ {[SpoolDir]})
+               ∖ {[SpoolDir]} : gset string) =
+           ((set_map UserDir (dom (gset uint64) σ.(messages))))) as ->.
+    { set_solver. }
+    rewrite big_opS_fmap; last first.
+    { rewrite /UserDir. intros ?? Heq. apply string_app_inj, uint64_to_string_inj in Heq. auto. }
+    iDestruct (big_sepM_dom with "Hdirlocks") as "Hdirlocks".
+    iDestruct (big_sepM_sepM with "[Hdirlocks Hmsgs]") as "Hmsgs".
+    { iFrame. }
+    iDestruct (big_sepM_sepM with "[Hmsgs]") as "Hmsgs".
+    { iFrame. iFrame "HΓ'". }
+    iApply (big_sepM_mono with "Hmsgs").
+    iIntros (k x Hlookup) "((H1&H2)&H3)".
+    iDestruct "H3" as %Hlookup'.
+    destruct Hlookup' as (γ'&?).
+    iDestruct "H1" as (??) "(_&(?&?&?))".
+    iExists _, _.
+    iSplitL ""; eauto.
+    iSplitL ""; eauto.
+    iFrame. auto.
   }
   { admit. }
   { iIntros (??) "(H1&H2)". iDestruct "H1" as (Hinv) "(H&Hstarter)".
